<section xml:id="section-change-of-variables">
  <title>Change of Variables</title>
  <p>
    Substitution was very useful for single variable integration. In
    the <m>e^{-x^2}</m> example, we did single-variable substitution
    in <m>y</m>, treating <m>x</m> as a constant. One might think
    that since we do iterated integrals, single variable substitution
    is sufficient. However, treating substitution in several
    variables holistically turns out to be very useful and powerful.
  </p>
  <p>
    Let's review single variable substitution, formalizing the
    language and showing the way forward for higher dimensions.
    Consider a single variable integral.
    <me>
      \int_{x=a}^{x=b} f(x) dx
    </me>
  </p>
  <p>
    Typically, we substitute <m>u = g(x)</m> using some
    <em>invertible</em> function <m>g</m>. Then we have <m>du =
    g^\prime(x) dx</m> and we try to change all the <m>x</m> variables
    to <m>u</m> variables with some algebra. We also change the
    bounds, starting from <m>u = g(a)</m> to <m>u = g(b)</m>. In this
    process, the old variable is the <em>domain</em> of the
    transformation and the new variable is the <em>range</em>.
  </p>
  <p>
    However, for several variables we're going other direction. We
    want the starting variables <m>x_i</m> to be the range. We do
    have one example from single variable calculus in this style;
    trigonometric substitution, such as <m>x = a \sin \theta</m>, have
    the original variable as the output of the transformation.
  </p>
  <p>
    Therefore, in the single variable case, introduce a new variable
    <m>u</m> by <m>x = h(u)</m> for some <em>invertible</em> function
    <m>h</m>. Then <m>dx = h^\prime(u) du</m> and the bounds become
    <m>h^{-1}(a)</m> and <m>h^{-1}(b)</m>. We get a new integral in
    the variable <m>u</m>.
    <me>
      \int_{u=h^{-1}(a)}^{u=h^{-1}(b)} f(h(u)) h^\prime(u) du
    </me>
  </p>
  <p>
    The key relationship here is <m>dx = h^\prime(u) du</m>: the
    derivative tells us the relationships between the differential
    terms. In Calculus III, we did all that work on extending the
    notion of the derivative. We came to the conclusion that the
    derivative measures (in local coordinates) the best linear
    approximation to the function. In one variable, that was just
    multiplication by a number. In several variables, though, that
    linear approximation was a matrix, called the Jacobian matrix.
    Let's recall the definition.
  </p>
  <definition>
    <statement>
      <p>
        Let <m>F: \RR^n \rightarrow \RR^n</m> be a function on
        <m>n</m> variables, <m>x_1, \ldots, x_n</m>. We can write
        <m>F</m> as its component functions <m>F_1, \ldots, F_n</m>.
        Then the Jacobian Matrix of <m>F</m> is the matrix of all
        partial derivatives.
        <me>
          J(F) = \left( \begin{matrix} \frac{\del F_1}{\del x_1} \amp
          \frac{\del F_1}{\del x_2} \amp \ldots \amp \frac{\del
          F_1}{\del x_n} \\ \frac{\del F_2}{\del x_1} \amp \frac{\del
          F_2}{\del x_2} \amp \ldots \amp \frac{\del F_2}{\del x_n} \\
          \vdots \amp \vdots \amp \vdots \amp \vdots \\ \frac{\del
          F_n}{\del x_1} \amp \frac{\del F_n}{\del x_2} \amp \ldots
          \amp \frac{\del F_n}{\del x_n} \end{matrix} \right)
        </me>
      </p>
      <p>
        The determinant <m>\det J(F)</m> is called the Jacobian of the
        function and is often written <m>|J(F)|</m>. Note that the
        notation <m>|\cdot|</m> is a reminder to take a determinant;
        it is <term>not</term> an absolute value. The Jacobian is
        often negative.
      </p>
    </statement>
  </definition>
  <p>
    From the single variable case <m>dx = h^\prime(u) du</m>, the
    Jacobian is part of the new differential <m>du</m>. If we start
    with variables <m>x_1, x_2, \ldots, x_n</m> and we have a function
    <m>F: \RR^n \rightarrow \RR^n</m> that has <m>x_i</m> as it output
    (the original variables are the range of the transformation), we
    can write <m>x_1 = F_1(u_1, \ldots, u_n)</m>, <m>x_2 = F_2(u_1,
    \ldots, u_n)</m> up to <m>x_n = F_n(u_1, \ldots, u_n)</m>. The
    Jacobian determines the relationship between the differential in
    these variables.
    <me>
      dx_1 dx_2 \ldots dx_n = |J(F)| du_1 du_2 \ldots du_n
    </me>
  </p>
  <p>
    We can interpret the Jacobian as the change in
    area/volume/hyper-volume due to the change in variables. Its
    appearance in the integral makes sense with this interpretation:
    the integral is measureing area/volume/hyper-volume, so when we
    change variables, we need a term that keeps track of the relative
    change in area/volume/hypervolume.
  </p>
  <example>
    <statement>
      <p>
        Let <m>(x,y) = F(u,v) = (3u, 4v)</m>. Then we have
        <md>
          <mrow>
            \frac{\del F_1}{\del u} \amp = 3
          </mrow>
          <mrow>
            \frac{\del F_1}{\del v} \amp = 0
          </mrow>
          <mrow>
            \frac{\del F_2}{\del u} \amp = 0
          </mrow>
          <mrow>
            \frac{\del F_2}{\del v} \amp = 4
          </mrow>
          <mrow>
            J(F) \amp = \left( \begin{matrix} 3 \amp 0
          </mrow>
          <mrow>
            0 \amp 5 \end{matrix} \right)
          </mrow>
          <mrow>
            |J(F)| \amp = (3)(4) - (0)(0) = 12
          </mrow>
          <mrow>
            dx dy \amp = 12 du dv
          </mrow>
        </md>
      </p>
      <p>
        The function is a dialation by <m>3</m> in <m>u</m> and by
        <m>4</m> in <m>v</m>, so the effect on area is multiplication
        by <m>12</m>, which makes sense. The function is linear
        already, to the linear approximation is constant: it is
        exactly the function itself.
      </p>
    </statement>
  </example>
  <example>
    <statement>
      <p>
        Let <m>(x,y) = F(u,v) = (u^2, v)</m>.
        <md>
          <mrow>
            \frac{\del F_1}{\del u} \amp = 2u
          </mrow>
          <mrow>
            \frac{\del F_1}{\del v} \amp = 0
          </mrow>
          <mrow>
            \frac{\del F_2}{\del u} \amp = 0
          </mrow>
          <mrow>
            \frac{\del F_2}{\del v} \amp = 1
          </mrow>
          <mrow>
            J(F) \amp = \left( \begin{matrix} 2u \amp 0
          </mrow>
          <mrow>
            0 \amp 1 \end{matrix} \right)
          </mrow>
          <mrow>
            |J(F)| \amp = 2u
          </mrow>
          <mrow>
            dx dy \amp = 2u du dv
          </mrow>
        </md>
      </p>
      <p>
        This Jacobian isn't constant. This is a stretch in <m>u</m>,
        the but effect is exagerated away from the origin due to the
        square term. Therefore, as <m>u</m> get larger, the stretch
        effect is greater. The Jacobian reflects that.
      </p>
    </statement>
  </example>
  <example>
    <statement>
      <p>
        Let <m>(x,y) = F(r,\theta) = (r \cos \theta, r \sin
        \theta)</m>. (Polar coordinates!)
        <md>
          <mrow>
            \frac{\del F_1}{\del r} \amp = \cos \theta
          </mrow>
          <mrow>
            \frac{\del F_1}{\del \theta} \amp = -r\sin \theta
          </mrow>
          <mrow>
            \frac{\del F_2}{\del r} \amp = \sin \theta
          </mrow>
          <mrow>
            \frac{\del F_2}{\del \theta} \amp = r \cos \theta
          </mrow>
          <mrow>
            J(F) \amp = \left( \begin{matrix} \cos \theta \amp - r
            \sin \theta
          </mrow>
          <mrow>
            \sin \theta \amp r \cos \theta \end{matrix} \right)
          </mrow>
          <mrow>
            |J(F)| \amp = r
          </mrow>
          <mrow>
            dx dy \amp = r dr d\theta
          </mrow>
        </md>
      </p>
      <p>
        This Jacobian shows that the radius term gives the effect on
        area. This make sense: for larger circles, the differential
        area is part of a larger arc.
      </p>
    </statement>
  </example>
  <example>
    <statement>
      <p>
        Let <m>(x,y) = F(u,v) = (u, uv)</m>. This is the change in
        variables we used in the <m>e^{-x^2}</m> example, now treated
        as a two-variable changes of variables.
        <md>
          <mrow>
            \frac{\del F_1}{\del u} \amp = 1
          </mrow>
          <mrow>
            \frac{\del F_1}{\del v} \amp = 0
          </mrow>
          <mrow>
            \frac{\del F_2}{\del u} \amp = v
          </mrow>
          <mrow>
            \frac{\del F_2}{\del v} \amp = u
          </mrow>
          <mrow>
            J(F) \amp = \left( \begin{matrix} 1 \amp 0
          </mrow>
          <mrow>
            v \amp u \end{matrix} \right)
          </mrow>
          <mrow>
            |J(F)| \amp = u
          </mrow>
          <mrow>
            dx dy \amp = u du dv
          </mrow>
        </md>
      </p>
    </statement>
  </example>
  <p>
    We can use a change of variables to help us with either the
    integrand or the region of integration. Sometime, as in the
    following examples, the same transformation helps both. When we
    are choosing a change of variables to simplify the region of
    integration, we are looking for a transformation where some of the
    bounding curves of the region become <m>u=c</m> or <m>v=c</m>. We
    need constant bounds in at least one of the variable to set up the
    iterated integral.
  </p>
  <example>
    <statement>
      <p>
        Let <m>D</m> be the region in the first quadrant between the
        lines <m>x+y = 1</m> and the line <m>x+y =2</m>. In the
        following integral, we want to simply the integrand and
        integrate over a simpler region if possible.
        <me>
          \int_D \cos \left( \frac{y-x}{y+x} \right) dA
        </me>
      </p>
      <p>
        To simplify the integrand, we can look for transformations
        where <m>u = x+y</m> and <m>v = x-y</m>. Inverting these
        (either by linear algebra, since the transformation is linear,
        or just by solving with conventional algebra), we get <m>x =
        \frac{u+v}{2}</m> and <m>y = \frac{u-v}{2}</m>.
      </p>
      <p>
        Then we look at the bounds. If we take <m>x+y=1</m> and
        replace <m>x</m> and <m>y</m>, we get <m>u=1</m>. Likewise,
        <m>x+y=2</m> is <m>u=2</m>. This is excellent, since we need
        at least one variable with constant bounds; we'll take
        <m>u</m> to be the variable of the outside integral. The
        other bounds are the axes, which we can express by the
        equations <m>y=0</m> and <m>x=0</m>. These turn into
        <m>u=v</m> and <m>u=-v</m>, respective. Therefore, the bounds
        of <m>v</m> will be these two lines: <m>v \in [u, -u]</m>.
      </p>
      <p>
        Finally, we calculate the Jacobian.
        <md>
          <mrow>
            x_u \amp = \frac{1}{2}
          </mrow>
          <mrow>
            x_v \amp = \frac{1}{2}
          </mrow>
          <mrow>
            y_u \amp = \frac{1}{2}
          </mrow>
          <mrow>
            y_v \amp = -\frac{1}{2}
          </mrow>
          <mrow>
            |J| \amp = -\frac{1}{2}
          </mrow>
          <mrow>
            dx dy \amp = \frac{1}{-2} du dv
          </mrow>
        </md>
      </p>
      <p>
        We have the new integrand, the new bounds and the Jacobian.
        We can proceed to the new integral.
        <md>
          <mrow>
            \int_D \cos \left( \frac{y-x}{y+x} \right) dA \amp =
            \int_1^2 \int_{-u}^u \cos \left( \frac{-v}{u} \right)
            \frac{-1}{2} dv du
          </mrow>
          <mrow>
            \amp = \frac{-1}{2} \int_1^2 \left. -\sin \left(
            \frac{-v}{u} \right) (-u) \right|_{-u}^{u} du
          </mrow>
          <mrow>
            \amp = \frac{-1}{2} \int_1^2 u (\sin (-1) - \sin(1)) du
          </mrow>
          <mrow>
            \amp = \frac{\sin (1) - \sin (-1)}{2} \left. \frac{u^2}{2}
            \right|_1^2
          </mrow>
          <mrow>
            \amp = \frac{\sin (1) - \sin (-1)}{2} (2 - \frac{1}{2}) =
            \frac{3(\sin(1) - \sin(-1))}{4}
          </mrow>
        </md>
      </p>
    </statement>
  </example>
  <example>
    <statement>
      <p>
        Let <m>D</m> be the region in the plane bounded by the curves
        <m>y = \frac{1}{x}</m>, <m>y = \frac{3}{x}</m>, <m>y = 3x</m>
        and <m>y = x</m>. Consider the following integral.
        <me>
          \int_D xy dA
        </me>
      </p>
      <p>
        The integrand is reasonable, so we will chose a substitution
        to changes the bounds. We want constant bounds in at least
        one variables. Here is one changes of variables which gets
        those constant bound: <m>(x,y) = F(u,v) = (uv,v)</m>. The
        lines <m>y=3x</m> and <m>y=x</m> become <m>v=3uv</m> and
        <m>v=uv</m>. Away from <m>v=0</m>, these lines are
        <m>u=\frac{1}{3}</m> and <m>u=1</m>, so we have constant
        bounds in <m>u</m> and we will treat <m>u</m> as the outside
        variable. (We are save with the assumption <m>v=0</m> since
        <m>v=y</m> and the region is disjoint from the <m>x</m>-axis,
        where <m>y=0</m>). The curves <m>y = \frac{1}{x}</m> and <m>y
        = \frac{3}{x}</m> become <m>v = \frac{1}{uv}</m> and <m>v =
        \frac{3}{uv}</m>, which simplify into <m>uv^2 =1</m> and
        <m>uv^2=3</m>. If we solve for <m>v</m> we get <m>v =
        \sqrt{\frac{1}{u}}</m> and <m>v = \sqrt{\frac{3}{u}}</m>.
        That means we can take <m>u \in [\frac{1}{3}, 3]</m> and <m>v
        \in \left[\sqrt{\frac{1}{u}}, \sqrt{\frac{3}{u}} \right]</m>.
        The integrand <m>xy</m> becomes <m>uv^2</m>.
        <md>
          <mrow>
            x_u \amp = v
          </mrow>
          <mrow>
            x_v \amp = u
          </mrow>
          <mrow>
            y_u \amp = 0
          </mrow>
          <mrow>
            y_v \amp = 1
          </mrow>
          <mrow>
            |J| \amp = (v)(1) - (u)(0) = v
          </mrow>
          <mrow>
            dx dy \amp = v du dv
          </mrow>
        </md>
      </p>
      <p>
        Then we complete the change of variables.
        <md>
          <mrow>
            \int_D xy dA \amp = \int_{\frac{1}{3}}^1
            \int_{\sqrt{\frac{1}{u}}}^{\sqrt{\frac{3}{u}}} uv^2 v dv
            du
          </mrow>
          <mrow>
            \amp = \int_{\frac{1}{3}}^1 \left. u\frac{v^4}{4}
            \right|_{\sqrt{\frac{1}{u}}}^{\sqrt{\frac{3}{u}}} du
          </mrow>
          <mrow>
            \amp = \int_{\frac{1}{3}}^1 \frac{u}{4} (\frac{9}{u^2} -
            \frac{1}{u^2}) du
          </mrow>
          <mrow>
            \amp = \int_{\frac{1}{3}}^1 \frac{-2}{u} du
          </mrow>
          <mrow>
            \amp = 2 \ln |u| \bigg|_{\frac{1}{3}}^1
          </mrow>
          <mrow>
            \amp = 2 \ln 1 - 2 \ln \frac{1}{3} = -2 \ln \frac{1}{3} =
            2 \ln 3
          </mrow>
        </md>
      </p>
      <p>
        For the same integral, we could have taken <m>y=v</m> and
        <m>x= \frac{u}{v}</m>. Under this transformation, the bounds
        become <m>u \in [1,3]</m> and <m>v \in [\sqrt{u},
        \sqrt{3u}]</m>. The Jacobian is now <m>\frac{1}{v}</m> and
        the integrand is <m>u</m>.
        <md>
          <mrow>
            \int_D xy dA \amp = \int_1^3 \int_{\sqrt{u}}^{\sqrt{3u}}
            \frac{1}{v} u dv du
          </mrow>
          <mrow>
            \amp = \int_1^3 u \ln |v| \bigg|_{\sqrt{u}}^{\sqrt{3u}} du
          </mrow>
          <mrow>
            \amp = \int_1^3 u (\ln |\sqrt{3u}| - \ln |\sqrt{u}|du
          </mrow>
          <mrow>
            \amp = \int_1^3 \frac{1}{2} (u \ln 3u - u \ln u) du
          </mrow>
          <mrow>
            \amp = \left. \frac{1}{2} \left(\frac{1}{4} u^2 (2 \ln 3u
            - 1) \frac{1}{3} - \frac{1}{4} u^2 (2 \ln u - 1) \right)
            \right|_1^3
          </mrow>
        </md>
      </p>
      <p>
        If we evaluate this, it will evaluate, eventually, to <m>2 \ln
        3</m>. However, the result is obviously more complicated.
        Different changes of variables can have very different effects
        on the integral; some will make it easier, some more
        difficult. Also, the answers from different change of
        variables can look quite differet, such as the expression
        above, while actually being the same value.
      </p>
      <p>
        As an aside, there is a simplification in the second version
        of this example that removes the complication. In the second
        last step, we could write <m>\ln 3u</m> as <m>\ln 3 + \ln
        u</m>.
        <md>
          <mrow>
            \amp = \int_1^3 \frac{1}{2} (u \ln 3u - u \ln u) du
          </mrow>
          <mrow>
            \amp = \frac{1}{2} \int_1^3 u (\ln 3 + \ln u - \ln u) du =
            \frac{1}{2} \int_1^3 u \ln 3 du
          </mrow>
          <mrow>
            \amp = \left. \frac{\ln 3}{2} \frac{u^2}{2} \right|_1^3 =
            \frac{\ln 3}{4} (9-1) = \frac{8 \ln 3}{4} = 2 \ln 3
          </mrow>
        </md>
      </p>
    </statement>
  </example>
  <example>
    <statement>
      <md>
        <mrow>
          \int_I f(x,y) dA \amp = \int_0^2 \int_3^6 \frac{3x+y}{2x-y}
          dy dx
        </mrow>
        <mrow>
          x \amp = \frac{u+v}{5}
        </mrow>
        <mrow>
          y \amp = \frac{2u-3v}{5}
        </mrow>
        <mrow>
          J \amp = \left( \begin{matrix} \frac{1}{5} \amp \frac{1}{5}
        </mrow>
        <mrow>
          \frac{2}{5} \amp \frac{-3}{5} \end{matrix} \right)
        </mrow>
        <mrow>
          |J| \amp = \frac{-1}{5}
        </mrow>
        <mrow>
          dy dx \amp = \frac{-1}{5} du dv
        </mrow>
        <mrow>
          \frac{3x+y}{2x-y} \amp = \frac{3u+3v+2u -3v}{2u + 2v -2u +
          3v} = \frac{5u}{5v} = \frac{u}{v}
        </mrow>
      </md>
      <p>
        The change of variables does indeed simplify the integrand,
        but what about the region of integration? We know <m>(x,y)
        \in [0,2] \times [3,6]</m>. Looking at the boundary
        lines<m>x=0</m> and <m>x=2</m> in the changes of variables
        gives <m>u+v=0</m> and <m>u+v-10</m>. Likewise, <m>y=3</m>
        and <m>y=6</m> give <m>2u-3v=15</m> and <m>2u-3v=30</m>. The
        resulting shape is a parallelogram with vertices <m>(9,1)</m>,
        <m>(12,-2)</m>, <m>(6,-6)</m> and <m>(3,-3)</m>. We would
        have to split up the domain of integration into three pieces
        to evaluate this; the result may be a much longer process than
        dealing with the original integral. Substitution may not
        always make things easier.
      </p>
    </statement>
  </example>
</section>
