<section xml:id="change-of-variables">
  <title>Change of Variables</title>
  <p>
    Substitution was very useful for single variable integration.
    In the <m>e^{-x^2}</m> example,
    we did single-variable substitution in <m>y</m>,
    treating <m>x</m> as a constant.
    One might think that since we do iterated integrals,
    single variable substitution is sufficient.
    However, treating substitution in several variables holistically turns out to be very useful and powerful.
  </p>
  <p>
    Let's review single variable substitution,
    formalizing the language and showing the way forward for higher dimensions.
    Consider a single variable integral.
    <me>
      \int_{x=a}^{x=b} f(x) dx
    </me>
  </p>
  <p>
    Typically, we substitute <m>u = g(x)</m> using some
    <em>invertible</em> function <m>g</m>.
    Then we have <m>du = g^\prime(x) dx</m> and we try to change all the <m>x</m> variables to <m>u</m> variables with some algebra.
    We also change the bounds, starting from <m>u = g(a)</m> to <m>u = g(b)</m>.
    In this process, the old variable is the <em>domain</em>
    of the transformation and the new variable is the <em>range</em>.
  </p>
  <p>
    However, for several variables we're going other direction.
    We want the starting variables <m>x_i</m> to be the range.
    We do have one example from single variable calculus in this style;
    trigonometric substitution, such as <m>x = a \sin \theta</m>,
    have the original variable as the output of the transformation.
  </p>
  <p>
    Therefore, in the single variable case,
    introduce a new variable <m>u</m> by <m>x = h(u)</m> for some
    <em>invertible</em> function <m>h</m>.
    Then <m>dx = h^\prime(u) du</m> and the bounds become
    <m>h^{-1}(a)</m> and <m>h^{-1}(b)</m>.
    We get a new integral in the variable <m>u</m>.
    <me>
      \int_{u=h^{-1}(a)}^{u=h^{-1}(b)} f(h(u)) h^\prime(u) du
    </me>
  </p>
  <p>
    The key relationship here is <m>dx = h^\prime(u) du</m>:
    the derivative tells us the relationships between the differential terms.
    In Calculus III, we did all that work on extending the notion of the derivative.
    We came to the conclusion that the derivative measures
    (in local coordinates)
    the best linear approximation to the function.
    In one variable, that was just multiplication by a number.
    In several variables, though,
    that linear approximation was a matrix,
    called the Jacobian matrix.
    Let's recall the definition.
  </p>
  <definition>
    <statement>
      <p>
        Let <m>F: \RR^n \rightarrow \RR^n</m> be a function on <m>n</m> variables,
        <m>x_1, \ldots, x_n</m>.
        We can write <m>F</m> as its component functions <m>F_1, \ldots, F_n</m>.
        Then the Jacobian Matrix of <m>F</m> is the matrix of all partial derivatives.
        <me>
          J(F) = \left( \begin{matrix} \frac{\del F_1}{\del x_1} \amp \frac{\del F_1}{\del x_2} \amp \ldots \amp \frac{\del F_1}{\del x_n} \\ \frac{\del F_2}{\del x_1} \amp \frac{\del F_2}{\del x_2} \amp \ldots \amp \frac{\del F_2}{\del x_n} \\ \vdots \amp  \vdots \amp  \vdots \amp  \vdots \\ \frac{\del F_n}{\del x_1} \amp \frac{\del F_n}{\del x_2} \amp \ldots \amp \frac{\del F_n}{\del x_n} \end{matrix} \right)
        </me>
      </p>
      <p>
        The determinant <m>\det J(F)</m> is called the Jacobian of the function and is often written <m>|J(F)|</m>.
        Note that the notation <m>|\cdot|</m> is a reminder to take a determinant;
        it is <term>not</term> an absolute value.
        The Jacobian is often negative.
      </p>
    </statement>
  </definition>
  <p>
    From the single variable case <m>dx = h^\prime(u) du</m>,
    the Jacobian is part of the new differential <m>du</m>.
    If we start with variables
    <m>x_1, x_2, \ldots,
    x_n</m> and we have a function
    <m>F: \RR^n \rightarrow \RR^n</m> that has <m>x_i</m> as it output
    (the original variables are the range of the transformation),
    we can write <m>x_1 = F_1(u_1, \ldots, u_n)</m>,
    <m>x_2 = F_2(u_1, \ldots, u_n)</m> up to <m>x_n = F_n(u_1, \ldots,
    u_n)</m>.
    The Jacobian determines the relationship between the differential in these variables.
    <me>
      dx_1 dx_2 \ldots dx_n = |J(F)| du_1 du_2 \ldots du_n
    </me>
  </p>
  <p>
    We can interpret the Jacobian as the change in area/volume/hyper-volume due to the change in variables.
    Its appearance in the integral makes sense with this interpretation:
    the integral is measureing area/volume/hyper-volume,
    so when we change variables,
    we need a term that keeps track of the relative change in area/volume/hypervolume.
  </p>
  <example>
    <statement>
      <p>
        Let <m>(x,y) = F(u,v) = (3u, 4v)</m>.
        Then we have
        <md>
          <mrow>\frac{\del F_1}{\del u} \amp  = 3</mrow>
          <mrow>\frac{\del F_1}{\del v} \amp  = 0</mrow>
          <mrow>\frac{\del F_2}{\del u} \amp  = 0</mrow>
          <mrow>\frac{\del F_2}{\del v} \amp  = 4</mrow>
          <mrow>J(F) \amp  = \left( \begin{matrix} 3 \amp  0</mrow>
          <mrow>0 \amp  5 \end{matrix} \right)</mrow>
          <mrow>|J(F)| \amp  = (3)(4) - (0)(0) = 12</mrow>
          <mrow>dx dy \amp  = 12 du dv</mrow>
        </md>
      </p>
      <p>
        The function is a dialation by <m>3</m> in <m>u</m> and by <m>4</m> in <m>v</m>,
        so the effect on area is multiplication by <m>12</m>, which makes sense.
        The function is linear already,
        to the linear approximation is constant:
        it is exactly the function itself.
      </p>
    </statement>
  </example>
  <example>
    <statement>
      <p>
        Let <m>(x,y) = F(u,v) = (u^2, v)</m>.
        <md>
          <mrow>\frac{\del F_1}{\del u} \amp  = 2u</mrow>
          <mrow>\frac{\del F_1}{\del v} \amp  = 0</mrow>
          <mrow>\frac{\del F_2}{\del u} \amp  = 0</mrow>
          <mrow>\frac{\del F_2}{\del v} \amp  = 1</mrow>
          <mrow>J(F) \amp  = \left( \begin{matrix} 2u \amp  0</mrow>
          <mrow>0 \amp  1 \end{matrix} \right)</mrow>
          <mrow>|J(F)| \amp  = 2u</mrow>
          <mrow>dx dy \amp  = 2u du dv</mrow>
        </md>
      </p>
      <p>
        This Jacobian isn't constant.
        This is a stretch in <m>u</m>,
        the but effect is exagerated away from the origin due to the square term.
        Therefore, as <m>u</m> get larger,
        the stretch effect is greater.
        The Jacobian reflects that.
      </p>
    </statement>
  </example>
  <example>
    <statement>
      <p>
        Let <m>(x,y) = F(r,\theta) = (r \cos \theta,
        r \sin \theta)</m>. (Polar coordinates!)
        <md>
          <mrow>\frac{\del F_1}{\del r} \amp  = \cos \theta</mrow>
          <mrow>\frac{\del F_1}{\del \theta} \amp  = -r\sin \theta</mrow>
          <mrow>\frac{\del F_2}{\del r} \amp  = \sin \theta</mrow>
          <mrow>\frac{\del F_2}{\del \theta} \amp  = r \cos \theta</mrow>
          <mrow>J(F) \amp  = \left( \begin{matrix} \cos \theta \amp  - r \sin \theta</mrow>
          <mrow>\sin \theta \amp  r \cos \theta \end{matrix} \right)</mrow>
          <mrow>|J(F)| \amp  = r</mrow>
          <mrow>dx dy \amp  = r dr d\theta</mrow>
        </md>
      </p>
      <p>
        This Jacobian shows that the radius term gives the effect on area.
        This make sense: for larger circles,
        the differential area is part of a larger arc.
      </p>
    </statement>
  </example>
  <example>
    <statement>
      <p>
        Let <m>(x,y) = F(u,v) = (u, uv)</m>.
        This is the change in variables we used in the <m>e^{-x^2}</m> example,
        now treated as a two-variable changes of variables.
        <md>
          <mrow>\frac{\del F_1}{\del u} \amp  = 1</mrow>
          <mrow>\frac{\del F_1}{\del v} \amp  = 0</mrow>
          <mrow>\frac{\del F_2}{\del u} \amp  = v</mrow>
          <mrow>\frac{\del F_2}{\del v} \amp  = u</mrow>
          <mrow>J(F) \amp  = \left( \begin{matrix} 1 \amp  0</mrow>
          <mrow>v \amp  u \end{matrix} \right)</mrow>
          <mrow>|J(F)| \amp  = u</mrow>
          <mrow>dx dy \amp  = u du dv</mrow>
        </md>
      </p>
    </statement>
  </example>
  <p>
    We can use a change of variables to help us with either the integrand or the region of integration.
    Sometime, as in the following examples,
    the same transformation helps both.
    When we are choosing a change of variables to simplify the region of integration,
    we are looking for a transformation where some of the bounding curves of the region become <m>u=c</m> or <m>v=c</m>.
    We need constant bounds in at least one of the variable to set up the iterated integral.
  </p>
  <example>
    <statement>
      <p>
        Let <m>D</m> be the region in the first quadrant between the lines <m>x+y = 1</m> and the line <m>x+y =2</m>.
        In the following integral,
        we want to simply the integrand and integrate over a simpler region if possible.
        <me>
          \int_D \cos \left( \frac{y-x}{y+x} \right) dA
        </me>
      </p>
      <p>
        To simplify the integrand,
        we can look for transformations where <m>u = x+y</m> and <m>v = x-y</m>.
        Inverting these
        (either by linear algebra,
        since the transformation is linear,
        or just by solving with conventional algebra),
        we get <m>x = \frac{u+v}{2}</m> and <m>y = \frac{u-v}{2}</m>.
      </p>
      <p>
        Then we look at the bounds.
        If we take <m>x+y=1</m> and replace <m>x</m> and <m>y</m>,
        we get <m>u=1</m>.
        Likewise, <m>x+y=2</m> is <m>u=2</m>.
        This is excellent,
        since we need at least one variable with constant bounds;
        we'll take <m>u</m> to be the variable of the outside integral.
        The other bounds are the axes,
        which we can express by the equations <m>y=0</m> and <m>x=0</m>.
        These turn into <m>u=v</m> and <m>u=-v</m>, respective.
        Therefore, the bounds of <m>v</m> will be these two lines:
        <m>v \in [u, -u]</m>.
      </p>
      <p>
        Finally, we calculate the Jacobian.
        <md>
          <mrow>x_u \amp  = \frac{1}{2}</mrow>
          <mrow>x_v \amp  = \frac{1}{2}</mrow>
          <mrow>y_u \amp  = \frac{1}{2}</mrow>
          <mrow>y_v \amp  = -\frac{1}{2}</mrow>
          <mrow>|J| \amp  = -\frac{1}{2}</mrow>
          <mrow>dx dy \amp  = \frac{1}{-2} du dv</mrow>
        </md>
      </p>
      <p>
        We have the new integrand, the new bounds and the Jacobian.
        We can proceed to the new integral.
        <md>
          <mrow>\int_D \cos \left( \frac{y-x}{y+x} \right) dA \amp  = \int_1^2 \int_{-u}^u \cos \left( \frac{-v}{u} \right) \frac{-1}{2} dv du</mrow>
          <mrow>\amp  = \frac{-1}{2} \int_1^2 \left. -\sin \left( \frac{-v}{u} \right) (-u) \right|_{-u}^{u} du</mrow>
          <mrow>\amp  = \frac{-1}{2} \int_1^2 u (\sin (-1) - \sin(1)) du</mrow>
          <mrow>\amp  = \frac{\sin (1) - \sin (-1)}{2} \left. \frac{u^2}{2} \right|_1^2</mrow>
          <mrow>\amp  = \frac{\sin (1) - \sin (-1)}{2} (2 - \frac{1}{2}) = \frac{3(\sin(1) - \sin(-1))}{4}</mrow>
        </md>
      </p>
    </statement>
  </example>
  <example>
    <statement>
      <p>
        Let <m>D</m> be the region in the plane bounded by the curves <m>y = \frac{1}{x}</m>,
        <m>y = \frac{3}{x}</m>, <m>y = 3x</m> and <m>y = x</m>.
        Consider the following integral.
        <me>
          \int_D xy dA
        </me>
      </p>
      <p>
        The integrand is reasonable,
        so we will chose a substitution to changes the bounds.
        We want constant bounds in at least one variables.
        Here is one changes of variables which gets those constant bound:
        <m>(x,y) = F(u,v) = (uv,v)</m>.
        The lines <m>y=3x</m> and <m>y=x</m> become <m>v=3uv</m> and <m>v=uv</m>.
        Away from <m>v=0</m>,
        these lines are <m>u=\frac{1}{3}</m> and <m>u=1</m>,
        so we have constant bounds in <m>u</m> and we will treat <m>u</m> as the outside variable. (We are save with the assumption <m>v=0</m> since <m>v=y</m> and the region is disjoint from the <m>x</m>-axis,
        where <m>y=0</m>).
        The curves <m>y = \frac{1}{x}</m> and <m>y = \frac{3}{x}</m> become
        <m>v = \frac{1}{uv}</m> and <m>v = \frac{3}{uv}</m>,
        which simplify into <m>uv^2 =1</m> and <m>uv^2=3</m>.
        If we solve for <m>v</m> we get
        <m>v = \sqrt{\frac{1}{u}}</m> and <m>v = \sqrt{\frac{3}{u}}</m>.
        That means we can take <m>u \in [\frac{1}{3}, 3]</m> and <m>v \in \left[\sqrt{\frac{1}{u}}, \sqrt{\frac{3}{u}} \right]</m>.
        The integrand <m>xy</m> becomes <m>uv^2</m>.
        <md>
          <mrow>x_u \amp  = v</mrow>
          <mrow>x_v \amp  = u</mrow>
          <mrow>y_u \amp  = 0</mrow>
          <mrow>y_v \amp  = 1</mrow>
          <mrow>|J| \amp  = (v)(1) - (u)(0) = v</mrow>
          <mrow>dx dy \amp  = v du dv</mrow>
        </md>
      </p>
      <p>
        Then we complete the change of variables.
        <md>
          <mrow>\int_D xy dA \amp  = \int_{\frac{1}{3}}^1 \int_{\sqrt{\frac{1}{u}}}^{\sqrt{\frac{3}{u}}} uv^2 v dv du</mrow>
          <mrow>\amp  = \int_{\frac{1}{3}}^1 \left. u\frac{v^4}{4} \right|_{\sqrt{\frac{1}{u}}}^{\sqrt{\frac{3}{u}}} du</mrow>
          <mrow>\amp  = \int_{\frac{1}{3}}^1 \frac{u}{4} (\frac{9}{u^2} - \frac{1}{u^2}) du</mrow>
          <mrow>\amp  = \int_{\frac{1}{3}}^1 \frac{-2}{u} du</mrow>
          <mrow>\amp  = 2 \ln |u| \bigg|_{\frac{1}{3}}^1</mrow>
          <mrow>\amp  = 2 \ln 1 - 2 \ln \frac{1}{3} = -2 \ln \frac{1}{3} = 2 \ln 3</mrow>
        </md>
      </p>
      <p>
        For the same integral,
        we could have taken <m>y=v</m> and <m>x= \frac{u}{v}</m>.
        Under this transformation,
        the bounds become <m>u \in [1,3]</m> and <m>v \in [\sqrt{u}, \sqrt{3u}]</m>.
        The Jacobian is now <m>\frac{1}{v}</m> and the integrand is <m>u</m>.
        <md>
          <mrow>\int_D xy dA \amp  = \int_1^3 \int_{\sqrt{u}}^{\sqrt{3u}} \frac{1}{v} u dv du</mrow>
          <mrow>\amp  = \int_1^3 u \ln |v| \bigg|_{\sqrt{u}}^{\sqrt{3u}} du</mrow>
          <mrow>\amp  = \int_1^3 u (\ln |\sqrt{3u}| - \ln |\sqrt{u}|du</mrow>
          <mrow>\amp  = \int_1^3 \frac{1}{2} (u \ln 3u - u \ln u) du</mrow>
          <mrow>\amp  = \left. \frac{1}{2} \left(\frac{1}{4} u^2 (2 \ln 3u - 1) \frac{1}{3} - \frac{1}{4} u^2 (2 \ln u - 1) \right) \right|_1^3</mrow>
        </md>
      </p>
      <p>
        If we evaluate this, it will evaluate,
        eventually, to <m>2 \ln 3</m>.
        However, the result is obviously more complicated.
        Different changes of variables can have very different effects on the integral;
        some will make it easier, some more difficult.
        Also, the answers from different change of variables can look quite differet,
        such as the expression above,
        while actually being the same value.
      </p>
      <p>
        As an aside,
        there is a simplification in the second version of this example that removes the complication.
        In the second last step,
        we could write <m>\ln 3u</m> as <m>\ln 3 + \ln u</m>.
        <md>
          <mrow>\amp  = \int_1^3 \frac{1}{2} (u \ln 3u - u \ln u) du</mrow>
          <mrow>\amp  = \frac{1}{2} \int_1^3 u (\ln 3 + \ln u - \ln u) du = \frac{1}{2} \int_1^3 u \ln 3 du</mrow>
          <mrow>\amp  = \left. \frac{\ln 3}{2} \frac{u^2}{2} \right|_1^3 = \frac{\ln 3}{4} (9-1) = \frac{8 \ln 3}{4} = 2 \ln 3</mrow>
        </md>
      </p>
    </statement>
  </example>
  <example>
    <statement>
      <md>
        <mrow>\int_I f(x,y) dA \amp  = \int_0^2 \int_3^6 \frac{3x+y}{2x-y} dy dx</mrow>
        <mrow>x \amp  = \frac{u+v}{5}</mrow>
        <mrow>y \amp  = \frac{2u-3v}{5}</mrow>
        <mrow>J \amp  = \left( \begin{matrix} \frac{1}{5} \amp  \frac{1}{5}</mrow>
        <mrow>\frac{2}{5} \amp  \frac{-3}{5} \end{matrix}
        \right)</mrow>
        <mrow>|J| \amp  = \frac{-1}{5}</mrow>
        <mrow>dy dx \amp  = \frac{-1}{5} du dv</mrow>
        <mrow>\frac{3x+y}{2x-y} \amp  = \frac{3u+3v+2u -3v}{2u + 2v -2u + 3v} =
        \frac{5u}{5v} = \frac{u}{v}</mrow>
      </md>
      <p>
        The change of variables does indeed simplify the integrand,
        but what about the region of integration?
        We know <m>(x,y) \in [0,2] \times [3,6]</m>.
        Looking at the boundary lines<m>x=0</m> and <m>x=2</m> in the changes of variables gives <m>u+v=0</m> and <m>u+v-10</m>.
        Likewise, <m>y=3</m> and <m>y=6</m> give <m>2u-3v=15</m> and <m>2u-3v=30</m>.
        The resulting shape is a parallelogram with vertices <m>(9,1)</m>,
        <m>(12,-2)</m>,
        <m>(6,-6)</m> and <m>(3,-3)</m>.
        We would have to split up the domain of integration into three pieces to evaluate this;
        the result may be a much longer process than dealing with the original integral.
        Substitution may not always make things easier.
      </p>
    </statement>
  </example>
</section>